rename "env" -> "ext"

Coq/Causality.v
@@ -10,14 +10,14 @@ Open Scope Z.
 Definition inp_until {A} (d : Z) (r1 r2 : inp A) : Prop :=
   forall z, Z.le z d -> r1 z = r2 z.
 
-Definition env_until (d : Z) (e1 e2 : env) : Prop :=
+Definition ext_until (d : Z) (e1 e2 : ext) : Prop :=
   inp_until d (fst e1) (fst e2) /\ inp_until d (snd e1) (snd e2).
 
 
 (* Semantic causality *)
 
 Definition causal (c : contract) : Prop :=
-  forall d r1 r2,  env_until (Z.of_nat d) r1 r2 -> (C[|c|]r1) d = (C[|c|]r2) d.
+  forall d r1 r2,  ext_until (Z.of_nat d) r1 r2 -> (C[|c|]r1) d = (C[|c|]r2) d.
 
 
 Lemma inp_until_adv {A} d t (r1 r2 : inp A): 
@@ -31,19 +31,19 @@ Proof.
 
 Qed.
 
-Lemma env_until_adv d t e1 e2: 
-    env_until d (adv_env t e1) (adv_env t e2) <-> env_until (t + d) e1 e2.
+Lemma ext_until_adv d t e1 e2: 
+    ext_until d (adv_ext t e1) (adv_ext t e2) <-> ext_until (t + d) e1 e2.
 Proof.
-  unfold env_until. repeat rewrite adv_env_obs. repeat rewrite adv_env_ch.
+  unfold ext_until. repeat rewrite adv_ext_obs. repeat rewrite adv_ext_ch.
   repeat rewrite inp_until_adv. reflexivity.
 Qed.
 
-Lemma env_until_adv_1 d r1 r2 : (1 <= d -> env_until d r1 r2 ->
-                        env_until (d - 1) (adv_env 1 r1) (adv_env 1 r2))%Z.
+Lemma ext_until_adv_1 d r1 r2 : (1 <= d -> ext_until d r1 r2 ->
+                        ext_until (d - 1) (adv_ext 1 r1) (adv_ext 1 r2))%Z.
 Proof.
   intros.
   assert (1 + (d - 1) = d)%Z by omega.
-  rewrite env_until_adv. rewrite H1. assumption.
+  rewrite ext_until_adv. rewrite H1. assumption.
 Qed.
 
 Lemma inp_until_le {A} d1 d2 (r1 r2 : inp A) : inp_until d1 r1 r2 ->  d2 <= d1 -> inp_until d2 r1 r2.
